IMLTT/typed/checked/ManualProofExamples.lean
@@ -1,0 +1,145 @@
+import IMLTT.typed.checked.Elaboration
+
+example : ε ⬝ 𝟙 ⊢ v(0) ∶ 𝟙 := HasType.var (IsType.unit_form IsCtx.empty)
+
+example : ε ⬝ 𝒩 ⬝ 𝟙 ⊢ v(0) ∶ 𝟙 := HasType.var
+  (IsType.unit_form (IsCtx.extend IsCtx.empty (IsType.nat_form IsCtx.empty)))
+
+
+example : ε ⬝ 𝒩 ⬝ 𝟙 ⊢ v(1) ∶ 𝒩 := by
+  let Γ := ε ⬝ 𝒩
+  have : Γ ctx := IsCtx.extend IsCtx.empty (IsType.nat_form IsCtx.empty)
+  have hΓ1 : Γ ⊢ 𝟙 type := IsType.unit_form this
+  have hwo : Γ ⊢ v(0) ∶ 𝒩 := HasType.var (IsType.nat_form IsCtx.empty)
+  exact HasType.weak hwo hΓ1
+
+example : ε ⬝ 𝟙 ⊢ (.refl 𝟙 v(0)) ∶ v(0) ≃[𝟙] v(0) := by
+  let Γ := ε ⬝ 𝟙
+  have hΓctx : Γ ctx := IsCtx.extend IsCtx.empty (IsType.unit_form IsCtx.empty)
+  have hΓ1type : Γ ⊢ 𝟙 type := IsType.unit_form hΓctx
+  have : Γ ⊢ v(0) ∶ 𝟙 := HasType.var (IsType.unit_form IsCtx.empty)
+  exact HasType.iden_intro hΓ1type this
+
+example (Γ : Ctx n) : (Γ ⊢ A type) -> (Γ ⬝ A ⊢ v(0) ∶ shift_tm A) := by
+  intro hAtype
+  apply HasType.var
+  exact hAtype
+
+example (Γ : Ctx n) : ∀ a : Tm n, (Γ ⊢ a ∶ 𝒩) → (Γ ⬝ 𝒩 ⊢ (shift_tm a) ≃[𝒩] v(0) type) := by
+  intro a ha
+  apply IsType.iden_form
+  · apply IsType.nat_form
+    apply IsCtx.extend
+    exact boundary_ctx_term ha
+    apply IsType.nat_form (boundary_ctx_term ha)
+  · have hΓNtype := IsType.nat_form (boundary_ctx_term ha)
+    exact weakening_term ha hΓNtype
+  · apply HasType.var
+    apply IsType.nat_form
+    exact boundary_ctx_term ha
+
+example (Γ : Ctx n) : ∀ a : Tm n, (Γ ⊢ a ∶ A) → (Γ ⬝ A ⊢ a⌊↑ₚidₚ⌋ ≃[A⌊↑ₚidₚ⌋] v(0) type) := by
+  intro a ha
+  have hae : Γ ⬝ A ⊢ a⌊↑ₚidₚ⌋ ∶ A⌊↑ₚidₚ⌋ := by
+    apply weakening_term
+    exact ha
+    exact boundary_term_type ha
+  apply IsType.iden_form
+  · exact boundary_term_type hae
+  · exact hae
+  · apply HasType.var
+    exact boundary_term_type ha
+
+example : (Γ ctx) -> Γ ⊢ Tm.lam 𝒩 v(0) ∶ Tm.pi 𝒩 𝒩 := by
+  intro hΓctx
+  apply HasType.pi_intro
+  apply HasType.var
+  apply IsType.nat_form
+  exact hΓctx
+
+example : (Γ ctx) -> Γ ⊢ Tm.app (Tm.lam 𝒩 v(0)) 𝓏 ∶ 𝒩 := fun hΓctx ↦
+  have h_pi := HasType.pi_intro (HasType.var (IsType.nat_form hΓctx));
+  HasType.pi_elim h_pi (HasType.nat_zero_intro hΓctx)
+
+example : (Γ ctx) -> Γ ⊢ (λ𝒩;v(0)) ◃ 𝓏 ∶ 𝒩 := by
+  intro hΓctx
+  have : Γ ⊢ λ𝒩;v(0) ∶ Π𝒩;𝒩 := by
+    apply HasType.pi_intro
+    apply HasType.var
+    apply IsType.nat_form
+    exact hΓctx
+  apply HasType.pi_elim this
+  exact HasType.nat_zero_intro hΓctx
+
+example : weaken ρ (.lam A b) =
+    .lam (weaken ρ A) (weaken (lift_weak_n 1 ρ) b) := rfl
+
+example : (Γ ctx) → (Γ ⬝ U ⊢ v(0) type) → (Γ ⬝ U ⬝ v(0) ⊢ v(0) ∶ v(1)) := by
+  intro hΓctx hv0type
+  apply HasType.var
+  exact hv0type
+
+example : ε ⬝ 𝒰 ⊢ v(0) type := by
+  apply boundary_type_eq_type' (A := v(0))
+  apply IsEqualType.univ_elim_eq
+  apply IsEqualTerm.var_eq
+  apply IsType.univ_form
+  exact IsCtx.empty
+
+example : ε ⬝ 𝒰 ⬝ v(0) ⊢ v(0) ∶ v(1) := by
+  apply HasType.var
+  apply boundary_type_eq_type' (A := v(0))
+  apply IsEqualType.univ_elim_eq
+  apply IsEqualTerm.var_eq
+  apply IsType.univ_form
+  exact IsCtx.empty
+
+theorem var_type_univ : ε ⬝ 𝒰  ⊢ v(0) type := by
+  apply boundary_type_eq_type' (A := v(0))
+  apply IsEqualType.univ_elim_eq
+  apply IsEqualTerm.var_eq
+  apply IsType.univ_form
+  exact IsCtx.empty
+
+--#imltt ε ⬝ (A : 𝒰) ⬝ (IdA : Π(a : A; A)) ⬝ (a : A) ⊢ (IdA a) : A
+example : ε ⬝ 𝒰 ⬝ (Πv(0);v(1)) ⬝ v(1) ⊢ v(1)◃v(0) ∶ v(2) := by
+  let Γ := ε ⬝ 𝒰 ⬝ (Πv(0);v(1)) ⬝ v(1)
+  have : ε ⬝ 𝒰 ⬝ (Πv(0);v(1)) ⬝ v(1) ⊢ v(1) ∶ (Πv(0+2);v(1+2)) := by
+    --apply HasType.weak
+    apply HasType.weak (B:= v(1)) (Γ := ε ⬝ 𝒰 ⬝ (Πv(0);v(1))) (i := 0) (A := (Πv(1);v(2)))
+    · apply HasType.var (A := Πv(0);v(1))
+      refine IsType.pi_form ?_ ?_
+      · exact var_type_univ
+      · apply boundary_type_eq_type' (A := v(1))
+        apply IsEqualType.univ_elim_eq
+        apply IsEqualTerm.weak_eq (B := v(0)) (Γ := ε ⬝ 𝒰) (i := 0) (A := 𝒰)
+        · aesop
+        · exact var_type_univ
+    · apply boundary_type_eq_type' (A := v(1))
+      apply IsEqualType.univ_elim_eq
+      apply IsEqualTerm.weak_eq (B := Πv(0);v(1)) (Γ := ε ⬝ 𝒰) (i := 0) (A := 𝒰)
+      · aesop
+      · refine IsType.univ_elim ?_
+        apply HasType.univ_pi
+        · aesop
+        · apply HasType.weak (B := v(0)) (Γ := ε ⬝ 𝒰) (i := 0) (A := 𝒰)
+          · aesop
+          · aesop
+  apply HasType.pi_elim this
+  apply HasType.var
+  apply boundary_type_eq_type' (A := v(1))
+  apply IsEqualType.univ_elim_eq
+  apply IsEqualTerm.weak_eq (i := 0) (B := Πv(0);v(1)) (Γ := ε ⬝ 𝒰) (A := 𝒰)
+  · aesop
+  · refine IsType.univ_elim ?_
+    apply HasType.univ_pi
+    · aesop
+    · apply HasType.weak (B := v(0)) (Γ := ε ⬝ 𝒰) (i := 0) (A := 𝒰)
+      · aesop
+      · aesop
+
+-- redundancy of rules
+example (hctx : Γ ctx) : Γ ⊢ 𝟙 ≡ 𝟙 type :=
+  IsEqualType.unit_form_eq hctx
+example (hctx : Γ ctx) : Γ ⊢ 𝟙 ≡ 𝟙 type :=
+  IsEqualType.univ_elim_eq <| IsEqualTerm.univ_unit_eq hctx
